Update complex C# test and start Java one

Source/IntegrationTests/TestFiles/LitTests/LitTest/comp/placeholders/complex/Interop/__default.java
@@ -1,0 +1,21 @@
+
+
+
+package Interop;
+
+import java.lang.Integer;
+import java.math.BigInteger;
+import dafny.TypeDescriptor;
+
+public class __default {
+  public static BigInteger Int32ToInt(Integer value) {
+    return BigInteger.valueOf(value);
+  }
+  public static DafnyStdLibs.Wrappers.Option<Integer> IntToInt32(BigInteger value) {
+    try {
+      return DafnyStdLibs.Wrappers.Option.create_Some(TypeDescriptor.intWithDefault(0), (Integer)value.intValueExact());
+    } catch(ArithmeticException e) {
+      return DafnyStdLibs.Wrappers.Option.create_None(TypeDescriptor.intWithDefault(0));
+    }
+  }
+}
