Source/IntegrationTests/TestFiles/LitTests/LitTest/comp/placeholders/complex/randomCSharp.dfy
@@ -1,25 +1,41 @@
 
 module RandomCSharp replaces DfyRandom {
   import CSharpSystem
+  import CSharpSystemTypes
   import Interop
   
   method GetRandomNat ... {
     // Ignore the ceiling parameter for now
     var random := new CSharpSystem.Random();
-    var resultInt32 := random.Next();
+    
+    var ceilingInt32 := Interop.IntToInt32(ceiling).GetOr(CSharpSystemTypes.Int32.MaxValue);
+    assert Interop.Int32ToInt(ceilingInt32) <= ceiling;
+    var resultInt32 := random.Next(Interop.IntToInt32(0).Extract(), ceilingInt32);
     var resultInt := Interop.Int32ToInt(resultInt32);
     return resultInt as nat;
   }
 }
 
 module Interop {
-  import CSharpSystemTypes
+  import opened CSharpSystemTypes
+  import opened DafnyStdLibs.Wrappers
   
-  function {:extern} Int32ToInt(value: CSharpSystemTypes.Int32): int
+  const int32MaxValue := 2147483647
+  
+  function {:extern} IntToInt32(value: int): Option<Int32>
+    ensures match IntToInt32(value) {
+      case None        => value > Int32ToInt(Int32.MaxValue)
+      case Some(int32) =>  Int32ToInt(int32) == value
+    }
+    ensures value <= int32MaxValue ==> IntToInt32(value).Some?
+    
+  function {:extern} Int32ToInt(value: Int32): int
 }
 
 module {:extern "System"} CSharpSystemTypes {
-  class {:extern "Int32" } Int32 { }
+  class {:extern "Int32" } Int32 {
+    static const {:extern} MaxValue: Int32 
+  }
 }
 
 module {:extern "System"} CSharpSystem {
@@ -29,7 +45,7 @@ module {:extern "System"} CSharpSystem {
   class {:extern "Random" } Random {
     constructor {:extern} () { }
     
-    method {:extern} Next() returns (r: Int32)
-      ensures Interop.Int32ToInt(r) >= 0
+    method {:extern} Next(minValue: Int32, maxValue: Int32) returns (r: Int32)
+      ensures var i := Interop.Int32ToInt(r); Interop.Int32ToInt(minValue) <= i && i < Interop.Int32ToInt(maxValue) 
   }
 }
