Source/IntegrationTests/TestFiles/LitTests/LitTest/comp/placeholders/complex/randomJava.dfy
@@ -1,0 +1,56 @@
+
+module RandomJava replaces DfyRandom {
+  import opened Interop
+  import opened JavaTypes
+  import opened JavaRest
+  
+  method GetRandomNat ... {
+    // Ignore the ceiling parameter for now
+    var random := new JavaRandom();
+    
+    var ceilingInt32 := IntToInt32(ceiling).GetOr(JavaInteger.MaxValue);
+    assert Int32ToInt(ceilingInt32) <= ceiling;
+    var resultInt32 := random.Next(ceilingInt32);
+    var resultInt := Int32ToInt(resultInt32);
+    return resultInt as nat;
+  }
+}
+
+module Interop {
+  import opened JavaTypes
+  import opened DafnyStdLibs.Wrappers
+  
+  const int32MaxValue := 2147483647
+  
+  function {:extern} IntToInt32(value: int): Option<Int32>
+    ensures match IntToInt32(value) {
+      case None        => value > Int32ToInt(JavaInteger.MaxValue)
+      case Some(int32) =>  Int32ToInt(int32) == value
+    }
+    ensures value <= int32MaxValue ==> IntToInt32(value).Some?
+    
+  function {:extern} Int32ToInt(value: Int32): int
+}
+  
+module {:extern ""} JavaTypes {
+  class {:extern "int" } Int32 {
+  }
+
+  class {:extern "java.lang.Integer" } JavaInteger {
+    // Would be nice to have an ensures here that equates it to 2147483647
+    // So we would not need Interop.int32MaxValue
+    static const {:extern "MAX_VALUE"} MaxValue: Int32 
+  }
+
+}
+module {:extern "java.util"} JavaRest {
+  import opened JavaTypes
+  import opened Interop
+  
+  class {:extern "Random" } JavaRandom {
+    constructor {:extern} () { }
+    
+    method {:extern "nextInt"} Next(bound: Int32) returns (r: Int32)
+      ensures var i := Int32ToInt(r); 0 <= i && i < Int32ToInt(bound) 
+  }
+}
