Source/IntegrationTests/TestFiles/LitTests/LitTest/comp/placeholders/complex/user.dfy
@@ -1,4 +1,4 @@
-// RUN: %baredafny run %args %s --build=%S/Build/build --input %S/random.dfy --input %S/randomCSharp.dfy --input %S/Interop.cs --spill-target-code > "%t"
+// RUN: %baredafny run %args %s --build=%S/Build/build --input %S/wrappers.dfy --input %S/random.dfy --input %S/randomCSharp.dfy --input %S/Interop.cs --spill-target-code > "%t"
 // RUN: %diff "%s.expect" "%t"
 
 method Main() {
